Setlec/Verify/Disc.lean
@@ -1029,7 +1029,8 @@ theorem whnfCoreBody_disc (ih : ScopedSim mode env f) (henv : EnvWF env)
           | .const c us =>
             if entry.native ∧ c = entry.ctor ∧ i < entry.numFields ∧
                 e'.getAppArgs.length = entry.numParams + entry.numFields ∧
-                us.length = entry.levelParams.length then
+                us.length = entry.levelParams.length ∧
+                entry.fireOk us = true then
               projCert C env d e' i entry.numParams >>= fun b =>
               if b then
                 (C : CoreFns CheckSM).whnfCore d
@@ -1046,7 +1047,8 @@ theorem whnfCoreBody_disc (ih : ScopedSim mode env f) (henv : EnvWF env)
           | .const c us =>
             if entry.native ∧ c = entry.ctor ∧ i < entry.numFields ∧
                 e'.getAppArgs.length = entry.numParams + entry.numFields ∧
-                us.length = entry.levelParams.length then
+                us.length = entry.levelParams.length ∧
+                entry.fireOk us = true then
               projCert G env d e' i entry.numParams >>= fun b =>
               if b then
                 (G : CoreFns CheckSM).whnfCore d
